ch07-quicksort/CLRS.Ch07.Partition.Impl.fsti
@@ -8,7 +8,7 @@ module CLRS.Ch07.Partition.Impl
 #lang-pulse
 
 open Pulse.Lib.Pervasives
-open CLRS.Ch07.Partition.Spec
+open CLRS.Ch07.Partition.Lemmas
 open CLRS.Common.SortSpec
 module A = Pulse.Lib.Array
 module GR = Pulse.Lib.GhostReference
