ch07-quicksort/CLRS.Ch07.Quicksort.Lemmas.fst
@@ -12,8 +12,7 @@
 *)
 module CLRS.Ch07.Quicksort.Lemmas
 
-open CLRS.Ch07.Partition.Spec
-open CLRS.Ch07.Quicksort.Spec
+open CLRS.Ch07.Partition.Lemmas
 open CLRS.Common.SortSpec
 module Seq = FStar.Seq
 
